TestsR.v
@@ -8,7 +8,7 @@ Require Import LibTactics.
 
 (* Require Export Stlc. *)
 Require Export Common LDef RecordsExt.
-Import P3Common LDEF Records.
+Import P3Common Records.
 
 Module RETests.
 
@@ -24,14 +24,29 @@ Notation k := (Id 6).
 Notation i1 := (Id 7).
 Notation i2 := (Id 8).
 
+(* Playing around with notations *)
+(*
+Example base1 : alookup a (aextend a (ttrue) nil) = Some ttrue.
+Proof. reflexivity. Qed.
+
+Notation "G ';;' 'val' x '\in' T" := (aextend x T G) (at level 40).
+
+Example base1c : alookup a (nil ;; val a \in TBool) = Some TBool.
+Proof. reflexivity. Qed.
+
+Notation "G 'has' 'val' x '\in' T" := (alookup x G = Some T) (at level 40).
+
+Example base1d : (nil ;; val a \in TBool) has val a \in TBool.
+Proof. reflexivity. Qed.
+*)
 (** [{ i1:A }] *)
 
-Example er1 : exists (t:ty), t = TRcd [(i1, A)].
+Example er1 : exists (t:ty), t = TRcd [(Lv i1 A)].
 Proof. eauto. Qed.
 
 (** [{ i1:A->B, i2:A }] *)
 Example er2 : exists (t:ty), t = 
-  TRcd [(i1, (TArrow A B)); (i2, A)].
+  TRcd [(Lv i1 (TArrow A B)); (Lv i2 A)].
 Proof. eauto. Qed.
 
 Definition substf_ok (sfunc:  id -> tm -> tm -> tm) :=
@@ -46,23 +61,33 @@ Definition substf_ok (sfunc:  id -> tm -> tm -> tm) :=
 Example subst_ok :substf_ok subst.
 Proof. unfold substf_ok. repeat split. Qed.
 
+Notation "Ls ';;;' x '\in' T" := (push_vdecl x T Ls) (at level 40).
+Notation "Fs ';;;' x = t"     := (push_vdef x t Fs) (at level 40).
+
+Example er2a : exists (t:ty), t = 
+  TRcd (nil ;;; i1 \in (TArrow A B) ;;; i2 \in A).
+Proof. eauto. Qed.
+
+Hint Constructors has_type rcd_has_type.
+
 Lemma typing_example_2 : 
   empty |- 
-    (tapp (tabs a (TRcd [(i1, (TArrow A A)); (i2, (TArrow B B))])
+    (tapp (tabs a (TRcd [(Lv i1 (TArrow A A)); (Lv i2 (TArrow B B))])
               (tproj (tvar a) i2))
-            (trcd [(i1, (tabs a A (tvar a))); (i2, (tabs a B (tvar a)))]) )
+            (trcd [(Fv i1 (tabs a A (tvar a))); (Fv i2 (tabs a B (tvar a)))]) )
     \in (TArrow B B).
-Proof. eauto 30 using extend_eq, eq_id. 
-       (* FIX EAUTO USAGE ABOVE *)
+Proof. 
+  (* info_eauto 20 using has_type, rcd_has_type, eq_id. *)
+  eauto 20 using eq_id. 
+  (* TBD: Figure out why eauto isn't taking the hints (above and before) *)
   eapply T_App.
     eapply T_Abs. eapply T_Proj.
       eapply T_Var.  eapply eq_id.
       reflexivity. 
-    eapply T_Rcd. eapply TR_Cons.
-      eapply T_Abs. eapply T_Var. eapply extend_eq.
-      eapply TR_Cons.
-        eapply T_Abs. eapply T_Var. eapply extend_eq.
-        eapply TR_Nil.
+    eapply T_Rcd.
+      eapply TR_Cons. eapply T_Abs. eapply T_Var. eapply extend_eq.
+      eapply TR_Cons. eapply T_Abs. eapply T_Var. eapply extend_eq.
+      eapply TR_Nil.
 Qed.
 
 (** Before starting to prove this fact (or the one above!), make sure
@@ -70,8 +95,8 @@ Qed.
 
 Example typing_nonexample : 
   ~ exists T,
-      (extend empty a (TRcd (cons (i2, (TArrow A A)) nil)))  |-
-               (trcd (cons (i1, (tabs a B (tvar a))) nil)) \in
+      (extend empty a (TRcd (cons (Lv i2 (TArrow A A)) nil)))  |-
+               (trcd (cons (Fv i1 (tabs a B (tvar a))) nil)) \in
                T.
   (* no T | a : { i2 : A->A } |- { i1 = λ a:B . a } : T *)
 Proof.
@@ -80,9 +105,8 @@ Proof.
 Example typing_nonexample_2 : forall y,
   ~ exists T,
     (extend empty y A) |-
-           (tapp (tabs a (TRcd (cons (i1, A) nil))
-                     (tproj (tvar a) i1))
-                   (trcd (cons (i1, (tvar y)) (cons (i2, (tvar y)) nil))) ) \in
+           (tapp (tabs a (TRcd [(Lv i1 A)]) (tproj (tvar a) i1))
+                 (trcd [(Fv i1 (tvar y)); (Fv i2 (tvar y))]) ) \in
            T.
   (* forall y, ~ exists T, y : A |- (λ a : { i1 : A} . a.i1) { i1 = y; i2 = y } : T *)
 Proof.
